---
title: Proof that $\exp(x)=\displaystyle\lim_{n\rightarrow\infty}\left(1+\frac{x}{n}\right)^{n}$
subtitle: A math-heavy but super elegant proof that I learnt
date: 2020-05-14 16:59:20 +0530
layout: default
keywords: math, exponentials
published: true
---

**Theorem 1.** $\exp(x)=\displaystyle\lim_{n\rightarrow\infty}\left(1+\frac{x}{n}\right)^{n}.$

**Proof.** Let $f(x)=\displaystyle\lim_{n\rightarrow\infty}\left(1+\frac{x}{n}\right)^{n}$ First, we'll neglect the limits and expand $f(x)$ using the binomial theorem.

$$f_{n}(x)=\sum_{k=0}^{n}\binom{x}{n}^{k}\frac{n!}{k!(n-k)!}$$

Now, we will increase $n$ to a sufficiently large value such that $\|f_{n}(x)-\exp(x)\|<\epsilon,\forall x.$ Once we find such a value, our proof will be complete.

$$|\exp(x)-f_{n}(x)|=\left|\sum_{k=0}^{n}\left(\frac{x^{k}}{k!}-\binom{x}{n}^{k}\frac{n!}{k!(n-k)!}\right)+\sum_{k=n+1}^{\infty}\frac{x^{k}}{k!}\right|.$$

We will make a slight change to the above equation and add a variable $m.$

$$|\exp(x)-f_{n}(x)|=\left|\sum_{k=0}^{m}\left(\frac{x^{k}}{k!}-\binom{x}{n}^{k}\frac{n!}{k!(n-k)!}\right)+\sum_{k=m+1}^{n}\left(\frac{x^{k}}{k!}-\binom{x}{n}^{k}\frac{n!}{k!(n-k)!}\right)+\sum_{k=n+1}^{\infty}\frac{x^{k}}{k!}\right|$$

$$\le\left|\sum_{k=0}^{m}\left(\frac{x^{k}}{k!}-\binom{x}{n}^{k}\frac{n!}{k!(n-k)!}\right)\right|+\left|\sum_{k=m+1}^{n}\left(\frac{x^{k}}{k!}-\binom{x}{n}^{k}\frac{n!}{k!(n-k)!}\right)\right|+\left|\sum_{k=n+1}^{\infty}\frac{x^{k}}{k!}\right|$$

$$\le\left|\sum_{k=0}^{m}\left(\frac{x^{k}}{k!}-\binom{x}{n}^{k}\frac{n!}{k!(n-k)!}\right)\right|+\left|\sum_{k=m+1}^{n}\frac{x^{k}}{k!}\right|+\left|\sum_{k=n+1}^{\infty}\frac{x^{k}}{k!}\right|$$

$$\le\left|\sum_{k=0}^{m}\left(\frac{x^{k}}{k!}-\binom{x}{n}^{k}\frac{n!}{k!(n-k)!}\right)\right|+\left|\sum_{k=m+1}^{\infty}\frac{x^{k}}{k!}\right|$$


We will look at the 2 terms individually, starting with the right.
Since $\displaystyle\frac{x^{k}}{k!}$ is eventually decreasing to 0, we can choose $m$ large enough so $\displaystyle\frac{x^{m}}{m!}<\displaystyle\frac{\epsilon}{4}$ and select an n larger than that.

$$\left|\sum_{k=m+1}^{\infty}\frac{x^{k}}{k!}\right|\le\frac{\epsilon}{4}\sum_{k=m+1}^{\infty}2^{-k}<\frac{\epsilon}{2}$$

Now, let's look at the left sum. The following expression will help us understand why the left sum is small.

$$\binom{x}{n}^{k}\frac{n!}{k!(n-k)!}=\frac{x^{k}(n(n-1)...(n-k+1)}{n^{k}k!}=\frac{x^{k}}{k!}\frac{(n(n-1)...(n-k+1)}{n^{k}}\approx\frac{x^{k}}{k!}$$

This approximation is valid as the terms almost cancel out.
Because of this each of the terms will be fairly small so hopefully we can make the entire sum small.
A clever observation is $n(n-m+1)\le (n-c)(n-k+1+c),$ $\forall k$ and positive $c$, this further means that

$$1\gt\frac{(n(n-1)\dots(n-k+1))}{n^k}\gt\left(\frac{n-m+1}{n}\right)^{m/2}\gt0$$

This further implies

$$\left|\sum_{k=0}^{m}\left(\frac{x^{k}}{k!}-\binom{x}{n}^{k}\frac{n!}{k!(n-k)!}\right)\right|\le\left|\sum_{k=0}^{m}\frac{x^{k}}{k!}\left(1-\left(\frac{n-m+1}{n}\right)^{m/2}\right)\right|=\left|\left(1-\left(\frac{n-m+1}{n}\right)^{m/2}\right)\sum_{k=0}^{m}\frac{x^{k}}{k!}\right|$$

From this, we know that $\exp(x)$ is finite everywhere, $\exists c$ such that $c$ is greater than all the partial sums of $\exp(x)$, therefore

$$\left|\left(1-\left(\frac{n-m+1}{n}\right)^{m/2}\right)\sum_{k=0}^{m}\frac{x^{k}}{k!}\right|\lt c\left(1-\left(\frac{n-m+1}{n}\right)^{m/2}\right)$$

We can now use Bernoulli's inequality to say that

Using this,

$$1>\left(\frac{n-m+1}{n}\right)^{m/2}=\left(1-\frac{m+1}{n}\right)^{m/2}>1-\frac{m^{2}+m}{2n}$$

$$c\left(1-\left(\frac{n-m+1}{n}\right)^{m/2}\right)<\frac{c(m^{2}+m)}{2n}$$

We fixed m earlier, and we can use this to find out how large $n$ must be, we get

$$n>\frac{c(m^{2}+m)}{\epsilon}$$

Ergo, putting all of this together


$$\left|\exp(x)-f_{n}(x)\right|\le\left|\sum_{k=0}^{m}\left(\frac{x^{k}}{k!}-\binom{x}{n}^{k}\frac{n!}{k!(n-k)!}\right)\right|+\left|\sum_{k=m+1}^{\infty}\frac{x^{k}}{k!}\right|<\epsilon$$

This shows that $f_{n}\rightarrow \exp(x)$ pointwise, in other words, $\exp(x)=f(x)$.

{: style="text-align: right" }
$\blacksquare$

---
